bsearch timing bounds fully proven

bedrock2/src/bedrock2Examples/bsearch.v
@@ -36,24 +36,11 @@ Import HList List. Require Import bedrock2.MetricLogging.
 Definition iterCost := {| instructions := 53; stores := 0; loads := 62; jumps := 2 |}.
 Definition endCost :=  {| instructions := 5; stores := 0; loads := 7; jumps := 1 |}.
 
-Definition nth(l: list word)(n: nat): word := List.nth n l (word.of_Z 0).
-
-Fixpoint In {A: Type} (a:A) (l:list A) : Prop :=
-    match l with
-      | nil => False
-      | cons b m => b = a \/ In a m
-end.
-
- Definition Sorted(l: list word): Prop :=
-    forall i j: nat, (i < j < List.length l)%nat ->
-                     word.unsigned (nth l i) <= word.unsigned (nth l j).
-
- Lemma sorted_in_window (l : list word) (target : word) (lower_indx : nat) (upper_indx : nat) :
-   In target l -> word.unsigned (nth l lower_indx) <= word.unsigned target <= word.unsigned (nth l lower_indx) -> exists target_indx,
-       Z.of_nat lower_indx <= Z.of_nat target_indx <= Z.of_nat upper_indx /\ nth l target_indx = target
- .
-   Proof. Admitted.
-
+ Definition msb (n : nat) := match n with
+                    | O => O
+                    | n => S (Nat.log2 n)
+ end.
+ 
 #[export] Instance spec_of_bsearch : spec_of "bsearch"%string := fun functions =>
   forall left right target xs R t m mc,
     sep (array scalar (word.of_Z 8) left xs) R m ->
@@ -61,7 +48,7 @@ end.
     WeakestPrecondition.call functions
       "bsearch"%string t m (left::right::target::nil)%list mc
       (fun t' m' rets mc' => t=t' /\ sep (array scalar (word.of_Z 8) left xs) R m' /\ 
-       (mc' - mc <= Z.of_nat (Nat.log2 (Datatypes.length xs)) * iterCost + endCost)%metricsH                               
+       (mc' - mc <= Z.of_nat (msb (Datatypes.length xs)) * iterCost + endCost)%metricsH                               
       ).
 
 
@@ -70,25 +57,35 @@ From coqutil.Macros Require Import symmetry.
 Import PrimitivePair.
 Require Import bedrock2.ZnWords.
 
-Lemma halvemod_by_shifts (n : word) (i : Z) : \_ n = 8 * i -> n ^>> /_ 4 ^<< /_ 3 = /_ (8*(i / 2)) .
+Lemma halvemod_by_shifts (n : word) (i : Z) : i >= 0 -> \_ n = 8 * i -> n ^>> /_ 4 ^<< /_ 3 = /_ (8*(i / 2)) .
 Proof.
-  intros.
-  assert (n = /_ (8 * i)) by ZnWords; subst n.
-
-  Admitted.
+  intros. ZnWords.
+ Qed.
 
 Lemma div2_sub (n : nat) : (n - S (Z.to_nat (Z.of_nat n / 2)) <= n / 2)%nat.
 Proof.
-Admitted.
+  replace (Z.to_nat (Z.of_nat n / 2)) with (n / 2)%nat by ((replace 2 with (Z.of_nat 2); try reflexivity); rewrite <- Nat2Z.inj_div; rewrite Nat2Z.id; trivial).
+  assert (n <= n/2 + S(n/2))%nat; try blia.
+  remember (Nat.even n) as ev; destruct ev.
+  - symmetry in Heqev; apply Nat.even_EvenT in Heqev; apply Nat.EvenT_Even in Heqev;
+    apply Nat.Even_double in Heqev; cbv [Nat.double] in *; rewrite Nat.div2_div in *; blia.
+  - rewrite <- Nat.negb_odd in Heqev; symmetry in Heqev; apply Bool.negb_false_iff in Heqev; assert (Hodd := Heqev);
+    rewrite <- Nat.even_succ in Heqev; apply Nat.even_EvenT in Heqev; apply Nat.EvenT_Even in Heqev;
+    apply Nat.Even_double in Heqev; cbv [Nat.double] in *; apply Nat.odd_OddT in Hodd; apply Nat.OddT_Odd in Hodd. 
+    assert (S (n / 2) + S (n / 2) = S n)%nat by (apply Nat.Odd_div2 in Hodd; repeat (rewrite Nat.div2_div in *); blia); blia.
+Qed.
 
-Lemma div2_sub_lies (n : nat) : (n - (Z.to_nat (Z.of_nat n / 2)) <= n / 2)%nat.
+Lemma div2_log (x y : nat) : (y > 0)%nat -> (x <= y / 2)%nat -> Z.of_nat (msb x) <= Z.of_nat (msb y) - 1.
 Proof.
-Admitted.
-
-
-Lemma div2_log (x y : nat) : (x <= y / 2)%nat -> Z.of_nat (Nat.log2 x) <= Z.of_nat (Nat.log2 y) - 1.
-Proof. Admitted.
-
+  intros; case (y / 2)%nat eqn:Hdiv.
+  - assert (x = 0)%nat by blia; destruct y; try blia; subst x; cbv [msb]; blia.
+  - destruct x; destruct y; cbv [msb]; try blia.
+    assert ( S (Nat.log2 (S x)) <= Nat.log2 (S y))%nat; try blia.
+    rewrite <- Nat.log2_double; try blia.
+    apply Nat.log2_le_mono; rewrite <- Nat.div2_div in Hdiv. 
+    assert (2 * S n <= S y)%nat; try blia; rewrite <- Hdiv; clear.
+    rewrite Nat.div2_odd; blia.
+Qed.
 
 Lemma bsearch_ok : program_logic_goal_for_function! bsearch.
 Proof.
@@ -102,7 +99,7 @@ Proof.
                                                 List.length xs = l)
                                                (fun T M LEFT RIGHT TARGET MC => T = t /\
                                                 sep (array scalar (word.of_Z 8) left xs) R M /\
-                                                (MC - mc <= (Z.of_nat (Nat.log2 (List.length xs))) * iterCost + endCost)%metricsH     
+                                                (MC - mc <= (Z.of_nat (msb (List.length xs))) * iterCost + endCost)%metricsH     
                                                )
                                                
         ) 
@@ -147,36 +144,22 @@ Proof.
       { SeparationLogic.ecancel_assumption. }
       { subst.
         subst metrics mc'0 metrics'0 mc'.
-        apply halvemod_by_shifts in length_rep as len_div2.
-        subst mid.  clear v0 H H0 H1 H2 H4 x0 x3 x5 x6 x7 x8 H6 left R m m0 M mc left'0 right target xs. 
+        apply halvemod_by_shifts in length_rep as len_div2; try ZnWords.
+        subst mid.  clear v0 H H0 H1 H2 x0 x3 x5 x6 x7 x8 H6 left R m m0 M mc left'0 right target xs. 
         subst x4. rewrite len_div2 in *; clear len_div2.
         rewrite length_skipn in H7.
-        replace (Z.div
-                                 (@word.unsigned 64 word
-                                    (@word.sub 64 word
-                                       (@word.add 64 word x1
-                                          (@word.of_Z 64 word
-                                             (Z.mul 8 (Z.div (Z.of_nat (@Datatypes.length (@word.rep 64 word) x)) 2)))) x1))
-                                 (@word.unsigned 64 word (@word.of_Z 64 word 8))) with
-          (Z.of_nat (Datatypes.length x) / 2)
-          in H7.
+        replace (Z.div (@word.unsigned 64 word (@word.sub 64 word (@word.add 64 word x1 (@word.of_Z 64 word
+        (Z.mul 8 (Z.div (Z.of_nat (@Datatypes.length (@word.rep 64 word) x)) 2)))) x1)) (@word.unsigned 64 word (@word.of_Z 64 word 8))) with
+          (Z.of_nat (Datatypes.length x) / 2) in H7.
         2: {
-          replace (@word.sub 64 word
-                                       (@word.add 64 word x1
-                                          (@word.of_Z 64 word
-                                             (Z.mul 8 (Z.div (Z.of_nat (@Datatypes.length (@word.rep 64 word) x)) 2)))) x1) with ((@word.of_Z 64 word
-                                             (Z.mul 8 (Z.div (Z.of_nat (@Datatypes.length (@word.rep 64 word) x)) 2)))) by ZnWords.
+          replace (@word.sub 64 word (@word.add 64 word x1 (@word.of_Z 64 word
+          (Z.mul 8 (Z.div (Z.of_nat (@Datatypes.length (@word.rep 64 word) x)) 2)))) x1) with
+          ((@word.of_Z 64 word (Z.mul 8 (Z.div (Z.of_nat (@Datatypes.length (@word.rep 64 word) x)) 2)))) by ZnWords.
           replace (\_ (/_ (8 * (Z.of_nat (Datatypes.length x) / 2)))) with (8 * (Z.of_nat (Datatypes.length x) / 2)) by ZnWords.
           rewrite Z.mul_comm; rewrite Z_div_mult; ZnWords.
         }
-        
-        assert (H:= div2_sub (Datatypes.length x)).
-        apply div2_log in H.
-
-        destruct mc0.
-        
-        applyAddMetrics H7. cbv [iterCost endCost] in *.
-        solve_MetricLog.
+        assert (H:= div2_sub (Datatypes.length x)); apply div2_log in H; try ZnWords.
+        destruct mc0; applyAddMetrics H7; cbv [iterCost endCost] in *; solve_MetricLog.                                                                                                     
       }
     }
     (* second branch of the if, very similar goals... *)
@@ -197,259 +180,35 @@ Proof.
       { SeparationLogic.ecancel_assumption. }
       { subst.
         subst metrics mc'0 metrics'0 mc'.
-        apply halvemod_by_shifts in length_rep as len_div2.
+        apply halvemod_by_shifts in length_rep as len_div2; try ZnWords.
         subst mid.  
         subst x4. rewrite len_div2 in *; clear len_div2.
-        clear v0 H H0 H1 H2 H4 x0 x3 x6 x7 x8 H6 left R m m0 M mc right target xs.
-
+        clear v0 H H0 H1 H2 x0 x3 x6 x7 x8 H6 left R m m0 M mc right target xs.
         rewrite List.firstn_length_le in H7.
         2: {
-          replace (@word.sub 64 word
-                                       (@word.add 64 word x1
-                                          (@word.of_Z 64 word
-                                             (Z.mul 8 (Z.div (Z.of_nat (@Datatypes.length (@word.rep 64 word) x)) 2)))) x1) with ((@word.of_Z 64 word
-                                             (Z.mul 8 (Z.div (Z.of_nat (@Datatypes.length (@word.rep 64 word) x)) 2)))) by ZnWords.
+          replace (@word.sub 64 word (@word.add 64 word x1 (@word.of_Z 64 word
+          (Z.mul 8 (Z.div (Z.of_nat (@Datatypes.length (@word.rep 64 word) x)) 2)))) x1) with
+          ((@word.of_Z 64 word (Z.mul 8 (Z.div (Z.of_nat (@Datatypes.length (@word.rep 64 word) x)) 2)))) by ZnWords.
           replace (\_ (/_ (8 * (Z.of_nat (Datatypes.length x) / 2)))) with (8 * (Z.of_nat (Datatypes.length x) / 2)) by ZnWords.
           rewrite Z.mul_comm; rewrite Z_div_mult; ZnWords.
         }
-        
-
-        replace (Z.div
-                                 (@word.unsigned 64 word
-                                    (@word.sub 64 word
-                                       (@word.add 64 word x1
-                                          (@word.of_Z 64 word
-                                             (Z.mul 8 (Z.div (Z.of_nat (@Datatypes.length (@word.rep 64 word) x)) 2)))) x1))
-                                 (@word.unsigned 64 word (@word.of_Z 64 word 8))) with
-          (Z.of_nat (Datatypes.length x) / 2)
-          in H7.
+        replace (Z.div (@word.unsigned 64 word (@word.sub 64 word (@word.add 64 word x1 (@word.of_Z 64 word
+        (Z.mul 8 (Z.div (Z.of_nat (@Datatypes.length (@word.rep 64 word) x)) 2)))) x1)) (@word.unsigned 64 word (@word.of_Z 64 word 8))) with
+          (Z.of_nat (Datatypes.length x) / 2) in H7.
         2: {
-          replace (@word.sub 64 word
-                                       (@word.add 64 word x1
-                                          (@word.of_Z 64 word
-                                             (Z.mul 8 (Z.div (Z.of_nat (@Datatypes.length (@word.rep 64 word) x)) 2)))) x1) with ((@word.of_Z 64 word
-                                             (Z.mul 8 (Z.div (Z.of_nat (@Datatypes.length (@word.rep 64 word) x)) 2)))) by ZnWords.
+          replace (@word.sub 64 word (@word.add 64 word x1 (@word.of_Z 64 word
+          (Z.mul 8 (Z.div (Z.of_nat (@Datatypes.length (@word.rep 64 word) x)) 2)))) x1) with
+          ((@word.of_Z 64 word (Z.mul 8 (Z.div (Z.of_nat (@Datatypes.length (@word.rep 64 word) x)) 2)))) by ZnWords.
           replace (\_ (/_ (8 * (Z.of_nat (Datatypes.length x) / 2)))) with (8 * (Z.of_nat (Datatypes.length x) / 2)) by ZnWords.
           rewrite Z.mul_comm; rewrite Z_div_mult; ZnWords.
         }
-
         assert (H := div2_log (Z.to_nat (Z.of_nat (Datatypes.length x) / 2)) (Datatypes.length x)).
-   
-
-        destruct mc0.
-        
-        applyAddMetrics H7. cbv [iterCost endCost] in *.
+        destruct mc0; applyAddMetrics H7; cbv [iterCost endCost] in *.
         assert (Z.to_nat (Z.of_nat (Datatypes.length x) / 2) <= Datatypes.length x / 2)%nat by
         (replace 2 with (Z.of_nat 2); try reflexivity; rewrite Nat2Z.inj_le; rewrite Z2Nat.id; try rewrite Nat2Z.inj_div; ZnWords).                              
         solve_MetricLog.
       }
       Unshelve. exact (word.of_Z 5). } }
-
   repeat straightline. split; auto. (* postcondition *)
- 
+
 Qed.
-
- (*
-#[export] Instance spec_of_bsearch : spec_of "bsearch"%string := fun functions =>
-  forall left right target xs R t m mc,
-    sep (array scalar (word.of_Z 8) left xs) R m ->
-    \_ (right ^- left) = 8*Z.of_nat (Datatypes.length xs) ->
-    WeakestPrecondition.call functions
-      "bsearch"%string t m (left::right::target::nil)%list mc
-      (fun t' m' rets mc' => t=t' /\ sep (array scalar (word.of_Z 8) left xs) R m' /\ exists i, rets = (i::nil)%list /\
-      (Sorted xs -> List.In target xs -> nth xs (Z.to_nat (( \_ i -  \_ left) / 8)) = target) /\
-       (mc' - mc <= initCost + Z.of_nat (Nat.log2 (Datatypes.length xs)) * iterCost + endCost)%metricsH                               
-      ).
-
-
-From coqutil.Tactics Require Import eabstract letexists rdelta.
-From coqutil.Macros Require Import symmetry.
-Import PrimitivePair.
-Require Import bedrock2.ZnWords.
-
-Lemma bsearch_ok : program_logic_goal_for_function! bsearch.
-Proof.
-  repeat straightline.
-
-  refine (
-    tailrec (HList.polymorphic_list.cons _ (HList.polymorphic_list.cons _ HList.polymorphic_list.nil)) ("left"::"right"::"target"::nil)%list%string
-        (fun l xs R t m left right target mc => PrimitivePair.pair.mk
-                                               (sep (array scalar (word.of_Z 8) left xs) R m /\
-                                                \_ (right ^- left) = 8*Z.of_nat (Datatypes.length xs) /\
-                                                List.length xs = l)
-                                               (fun T M LEFT RIGHT TARGET MC => T = t /\
-                                                sep (array scalar (word.of_Z 8) left xs) R M /\
-                                                Sorted xs -> List.In target xs -> exists target_index,
-                                                ( \_ LEFT <= (Z.of_nat target_index) *  8 + \_ left <= \_ RIGHT /\ nth xs target_index = target) /\
-                                                (MC - mc <= (Z.of_nat (Nat.log2 l)) * iterCost + endCost)%metricsH     
-                                               )
-                                               
-        ) 
-        lt _ _ _ _ _ _ _);
-    cbn [reconstruct map.putmany_of_list HList.tuple.to_list
-         HList.hlist.foralls HList.tuple.foralls
-         HList.hlist.existss HList.tuple.existss
-         HList.hlist.apply  HList.tuple.apply
-         HList.hlist
-         List.repeat Datatypes.length
-         HList.polymorphic_list.repeat HList.polymorphic_list.length
-         PrimitivePair.pair._1 PrimitivePair.pair._2] in *.
-
-  { repeat straightline. }
-  { exact lt_wf. }
-  { eauto. }
-  { repeat straightline.
-    2: {  }
-
-    
-    2: solve [auto].  (* exiting loop *)
-    (* loop body *)
-    rename H2 into length_rep. subst br.
-    
-    seprewrite @array_address_inbounds;
-       [ ..|(* if expression *) exact eq_refl|letexists; letexists; split; [repeat straightline|]]. (* determines element *)
-    { ZnWords. }
-    { ZnWords. }
-    (* split if cases *) split; repeat straightline. (* code is processed, loop-go-again goals left behind *)
-    { repeat letexists. split; [repeat straightline|].
-      1:split.
-      2:split.
-      { SeparationLogic.ecancel_assumption. }
-      { ZnWordsL. }
-      { cleanup_for_ZModArith. reflexivity. }
-      split; repeat straightline.
-      2: SeparationLogic.seprewrite_in (symmetry! @array_address_inbounds) H6.
-      { ZnWordsL. }
-      { ZnWords. }
-      { ZnWords. }
-      { trivial. }
-      { SeparationLogic.ecancel_assumption. } }
-    (* second branch of the if, very similar goals... *)
-    { repeat letexists. split.
-      1:split.
-      2:split.
-      { SeparationLogic.ecancel_assumption. }
-      { ZnWordsL. }
-      { cleanup_for_ZModArith. reflexivity. }
-      split.
-      { ZnWordsL. }
-      repeat straightline.
-      subst x5. SeparationLogic.seprewrite_in (symmetry! @array_address_inbounds) H6.
-      { ZnWords. }
-      { ZnWords. }
-      { ZnWords. }
-      { SeparationLogic.ecancel_assumption. } } }
-  repeat straightline.
-  repeat apply conj; auto; []. (* postcondition *)
-  letexists. split.
-  { exact eq_refl. }
-  repeat(split).
-  { auto. }
-  { eauto. }
-
-  Unshelve.
-  all: exact (word.of_Z 0).
-
-  all:fail "remaining subgoals".
-Qed.
-*)
-
-(*
-
-#[export] Instance spec_of_bsearch : spec_of "bsearch"%string := fun functions =>
-  forall left right target xs R t m mc,
-    sep (array scalar (word.of_Z 8) left xs) R m ->
-    \_ (right ^- left) = 8*Z.of_nat (Datatypes.length xs) ->
-    WeakestPrecondition.call functions
-      "bsearch"%string t m (left::right::target::nil)%list mc
-      (fun t' m' rets mc' => t=t' /\ sep (array scalar (word.of_Z 8) left xs) R m' /\ exists i, rets = (i::nil)%list /\
-      ((*sorted*)False -> True)                                      
-      ).
-
-
-From coqutil.Tactics Require Import eabstract letexists rdelta.
-From coqutil.Macros Require Import symmetry.
-Import PrimitivePair.
-Require Import bedrock2.ZnWords.
-
-Lemma bsearch_ok : program_logic_goal_for_function! bsearch.
-Proof.
-  repeat straightline.
-
-  refine (
-    tailrec (HList.polymorphic_list.cons _ (HList.polymorphic_list.cons _ HList.polymorphic_list.nil)) ("left"::"right"::"target"::nil)%list%string
-        (fun l xs R t m left right target mc => PrimitivePair.pair.mk
-                                               (sep (array scalar (word.of_Z 8) left xs) R m /\
-                                                \_ (right ^- left) = 8*Z.of_nat (Datatypes.length xs) /\
-                                                List.length xs = l)
-                                               (fun T M LEFT RIGHT TARGET MC => T = t /\ sep (array scalar (word.of_Z 8) left xs) R M
-                                               )
-                                               
-        ) 
-        lt _ _ _ _ _ _ _);
-    cbn [reconstruct map.putmany_of_list HList.tuple.to_list
-         HList.hlist.foralls HList.tuple.foralls
-         HList.hlist.existss HList.tuple.existss
-         HList.hlist.apply  HList.tuple.apply
-         HList.hlist
-         List.repeat Datatypes.length
-         HList.polymorphic_list.repeat HList.polymorphic_list.length
-         PrimitivePair.pair._1 PrimitivePair.pair._2] in *.
-
-  { repeat straightline. }
-  { exact lt_wf. }
-  { eauto. }
-  { repeat straightline.
-    2: solve [auto].  (* exiting loop *)
-    (* loop body *)
-    rename H2 into length_rep. subst br.
-    
-    seprewrite @array_address_inbounds;
-       [ ..|(* if expression *) exact eq_refl|letexists; letexists; split; [repeat straightline|]]. (* determines element *)
-    { ZnWords. }
-    { ZnWords. }
-    (* split if cases *) split; repeat straightline. (* code is processed, loop-go-again goals left behind *)
-    { repeat letexists. split; [repeat straightline|].
-      1:split.
-      2:split.
-      { SeparationLogic.ecancel_assumption. }
-      { ZnWordsL. }
-      { cleanup_for_ZModArith. reflexivity. }
-      split; repeat straightline.
-      2: SeparationLogic.seprewrite_in (symmetry! @array_address_inbounds) H6.
-      { ZnWordsL. }
-      { ZnWords. }
-      { ZnWords. }
-      { trivial. }
-      { SeparationLogic.ecancel_assumption. } }
-    (* second branch of the if, very similar goals... *)
-    { repeat letexists. split.
-      1:split.
-      2:split.
-      { SeparationLogic.ecancel_assumption. }
-      { ZnWordsL. }
-      { cleanup_for_ZModArith. reflexivity. }
-      split.
-      { ZnWordsL. }
-      repeat straightline.
-      subst x5. SeparationLogic.seprewrite_in (symmetry! @array_address_inbounds) H6.
-      { ZnWords. }
-      { ZnWords. }
-      { ZnWords. }
-      { SeparationLogic.ecancel_assumption. } } }
-  repeat straightline.
-  repeat apply conj; auto; []. (* postcondition *)
-  letexists. split.
-  { exact eq_refl. }
-  repeat(split).
-  { auto. }
-  { eauto. }
-
-  Unshelve.
-  all: exact (word.of_Z 0).
-
-  all:fail "remaining subgoals".
-Qed.
-(* Print Assumptions bsearch_ok. *)
-(* Closed under the global context *)
-*)
